snap

io/Compile.IIO.To.ILang.fst
@@ -5,11 +5,11 @@ open FStar.Tactics.Typeclasses
 
 open Common
 open IO.Sig
+open IO
 open IIO
 open TC.Monitorable.Hist
 open Compile.ILang
 open TC.Checkable
-open TC.Trivialize
 
 class exportable (t : Type u#a) (pi:monitorable_prop) = {
   etype : Type u#a;
@@ -30,6 +30,105 @@ class importable (t : Type u#a) (pi:monitorable_prop) = {
   import : itype -> resexn t;
 }
 
+noeq
+type iio_lang_interface = {
+  ct : Type;
+  pt : Type;
+
+  vpi : monitorable_prop;
+
+  c1 : exportable pt vpi;
+  c2 : importable ct vpi;
+}
+
+let test_interface : iio_lang_interface = {
+  pt = unit -> IIO unit (fun h -> True) (fun h r lt -> True);
+  ct = (x:file_descr) -> IIO unit (fun h -> is_open x h) (fun h r lt -> is_open x (apply_changes h lt));
+
+  vpi = (fun _ _ _ -> true);
+
+  c1 = admit ();
+  c2 = admit ();
+}
+
+type iio_lang_ctx (i:iio_lang_interface) = i.ct
+type iio_lang_prog (i:iio_lang_interface) = iio_lang_ctx i -> i.pt
+
+let iio_lang_language : BeyondCriteria.language = {
+  interface = iio_lang_interface;
+
+  ctx = iio_lang_ctx;
+  pprog = iio_lang_prog;
+  whole = (i:iio_lang_interface & i.pt);
+
+  link = (fun #i p c -> (| i, p c |));
+  event_typ = IO.Sig.event;
+
+  beh = admit ()
+}
+
+val test_prog : iio_lang_prog test_interface
+let test_prog ctx () =
+  let fd = static_cmd Openfile "../Makefile" in
+  if Inl? fd then ctx (Inl?.v fd)
+  else ()
+
+noeq
+type ilang_interface = {
+  pt : Type;
+  ct : Type;
+
+  vpi : monitorable_prop;
+}
+
+type ilang_ctx (i:ilang_interface) = i.ct
+type ilang_prog (i:ilang_interface) = ilang_ctx i -> i.pt
+
+let ilang_language : BeyondCriteria.language = {
+  interface = ilang_interface;
+
+  ctx = ilang_ctx;
+  pprog = ilang_prog;
+  whole = (i:ilang_interface & i.pt);
+
+  link = (fun #i p c -> (| i, p c |));
+  event_typ = IO.Sig.event;
+
+  beh = admit ();
+}
+
+let comp_int (i:iio_lang_interface) : ilang_interface = {
+    pt = resexn i.c1.etype;
+    ct = i.c2.itype;
+    vpi = i.vpi;
+}
+
+let compiler_pprog (#i:iio_lang_interface) (p:iio_lang_language.pprog i) : ilang_language.pprog (comp_int i) = fun c -> 
+    match i.c2.import c with
+    | Inl c' -> begin 
+      let (| _, pt |) = iio_lang_language.link #i p c' in
+      Inl (i.c1.export pt)
+    end
+    | Inr err -> Inr err
+
+let phase1 : BeyondCriteria.compiler = {
+  source = iio_lang_language;
+  target = ilang_language;
+
+  comp_int = comp_int;
+
+  compile_pprog = (fun #i p c -> 
+    match i.c2.import c with
+    | Inl c' -> begin 
+      let (| _, pt |) = iio_lang_language.link #i p c' in
+      (** WTF **)
+      assert False;
+      Inl (i.c1.export pt)
+    end
+    | Inr err -> Inr err);
+
+  rel_traces = admit ();
+}
 
 (** *** Exportable instances **)
 
